eliminate some axioms

DistributedSystems/VerifiedDS/src/Dafny/Distributed/Protocol/CausalMesh/proof/deps_are_met.dfy
@@ -113,6 +113,86 @@ lemma lemma_MergeCCacheEnsuresAllVersionAreMetOnAllServers(
     }
 } 
 
+// lemma lemma_MetaIsMetImpliesMetasBeforeItAreMet(
+//     b:Behavior<CMState>,
+//     i:int,
+//     meta:Meta,
+//     metas:set<Meta>
+// )
+//     requires i > 0
+//     requires IsValidBehaviorPrefix(b, i)
+//     // requires forall j :: 0 <= j < i ==> CMNext(b[j], b[j+1])
+//     requires CMNext(b[i-1], b[i])
+//     requires MetaValid(meta)
+//     requires AVersionIsMetOnAllServers(b, i, meta.key, meta.vc)
+//     requires forall j :: 0 < j <= i ==> AllWriteDepsAreMet(b, j)
+//     requires forall j :: 0 <= j < i ==> ServerNextDoesNotDecreaseVersions(b[j], b[j+1])
+//     requires forall m :: m in metas ==> MetaValid(m) && (VCHappendsBefore(m.vc, meta.vc) || VCEq(m.vc, meta.vc))
+//     ensures forall m :: m in metas ==> AVersionIsMetOnAllServers(b, i, m.key, m.vc)
+//     ensures forall m :: m in metas ==> AllVersionsInDepsAreMetOnAllServers(b, i, m.deps)
+// {
+//     reveal_AllVersionsInDepsAreMetOnAllServers();
+//     forall m | m in metas 
+//         ensures AVersionIsMetOnAllServers(b, i, m.key, m.vc);
+//         ensures AllVersionsInDepsAreMetOnAllServers(b, i, m.deps)
+//     {
+//         assert VCHappendsBefore(m.vc, meta.vc) || VCEq(m.vc, meta.vc);
+//         lemma_MetaIsMetImpliesAllPreviousMetasAreMet(b, i, meta, m);
+//         assert AVersionIsMetOnAllServers(b, i, m.key, m.vc);
+//         assert i > 0;
+//         assert IsValidBehaviorPrefix(b, i);
+//         assert MetaValid(m);
+//         assert AVersionIsMetOnAllServers(b, i, m.key, m.vc);
+//         assert forall j :: 0 < j <= i ==> AllWriteDepsAreMet(b, j);
+//         lemma_MetaIsMetImpliesItsDepsAreMet(b, i, m);
+//         assert AllVersionsInDepsAreMetOnAllServers(b, i, m.deps);
+//         assert AVersionIsMetOnAllServers(b, i, m.key, m.vc);
+//     }
+// }
+
+lemma lemma_MetaIsMetImpliesMetasBeforeItAreMet2(
+    b:Behavior<CMState>,
+    i:int,
+    idx:int,
+    meta:Meta,
+    metas:set<Meta>
+)
+    requires i > 0
+    requires IsValidBehaviorPrefix(b, i)
+    // requires forall j :: 0 <= j < i ==> CMNext(b[j], b[j+1])
+    requires CMNext(b[i-1], b[i])
+    requires 0 <= idx < Nodes
+    
+    requires MetaValid(meta)
+    requires AVersionIsMetOnAllServers(b, i, meta.key, meta.vc)
+    requires forall j :: 0 < j <= i ==> AllWriteDepsAreMet(b, j)
+    requires forall j :: 0 <= j < i ==> ServerNextDoesNotDecreaseVersions(b[j], b[j+1])
+    requires forall m :: m in metas ==> MetaValid(m) && (VCHappendsBefore(m.vc, meta.vc) || VCEq(m.vc, meta.vc))
+    // requires forall m :: m in metas ==> m in b[i].servers[idx].s.icache[m.key]
+    requires forall m :: m in metas ==> AVersionOfAKeyIsMet(b[i].servers[idx].s.icache, b[i].servers[idx].s.ccache, m.key, m.vc)
+    ensures forall m :: m in metas ==> AVersionIsMetOnAllServers(b, i, m.key, m.vc)
+    ensures forall m :: m in metas ==> AllVersionsInDepsAreMetOnAllServers(b, i, m.deps)
+{
+    reveal_AllVersionsInDepsAreMetOnAllServers();
+    forall m | m in metas 
+        ensures AVersionIsMetOnAllServers(b, i, m.key, m.vc);
+        ensures AllVersionsInDepsAreMetOnAllServers(b, i, m.deps)
+    {
+        // lemma_BehaviorValidImpliesOneStepValid()
+        assert VCHappendsBefore(m.vc, meta.vc) || VCEq(m.vc, meta.vc);
+        lemma_MetaIsMetImpliesAllPreviousMetasAreMet(b, i, meta, m);
+        assert AVersionIsMetOnAllServers(b, i, m.key, m.vc);
+        assert i > 0;
+        assert IsValidBehaviorPrefix(b, i);
+        assert MetaValid(m);
+        assert AVersionIsMetOnAllServers(b, i, m.key, m.vc);
+        assert forall j :: 0 < j <= i ==> AllWriteDepsAreMet(b, j);
+        lemma_MetaIsMetImpliesItsDepsAreMet2(b, i, idx, m);
+        assert AllVersionsInDepsAreMetOnAllServers(b, i, m.deps);
+        assert AVersionIsMetOnAllServers(b, i, m.key, m.vc);
+    }
+}
+
 lemma lemma_VersionsAfterPullDepsAreMetOnAllServers(
     b:Behavior<CMState>,
     i:int,
@@ -125,6 +205,7 @@ lemma lemma_VersionsAfterPullDepsAreMetOnAllServers(
     requires 0 <= idx < Nodes
     requires DependencyValid(deps)
     requires forall j :: 0 < j <= i ==> AllWriteDepsAreMet(b, j)
+    requires forall j :: 0 <= j < i ==> ServerNextDoesNotDecreaseVersions(b[j], b[j+1])
     requires AllVersionsInDepsAreMetOnAllServers(b, i, deps)
     requires AllVersionsInCCacheAreMetOnAllServers(b, i, b[i].servers[idx].s.ccache)
     ensures var res := PullDeps2(b[i].servers[idx].s.icache, b[i].servers[idx].s.ccache, deps);
@@ -141,9 +222,9 @@ lemma lemma_VersionsAfterPullDepsAreMetOnAllServers(
     var domain := icache.Keys + deps.Keys;
 
     var todos := GetMetasOfAllDeps(icache, deps, map[], domain);
-    var todos1 := GetMetasOfAllDepsGlobalView(b, i, idx, icache, deps, map[], domain);
+    var todos1 := GetMetasOfAllDepsGlobalView2(b, i, idx, icache, deps, map[], domain);
     assert forall k :: k in todos1 ==> AVersionIsMetOnAllServers(b, i, k, todos1[k].vc) && AllVersionsInDepsAreMetOnAllServers(b, i, todos1[k].deps);
-    lemma_GetMetasOfAllDepsGlobalViewEqualsToGetMetasOfAllDeps(b, i, idx, icache, deps, map[], domain);
+    lemma_GetMetasOfAllDepsGlobalViewEqualsToGetMetasOfAllDeps2(b, i, idx, icache, deps, map[], domain);
     assert todos == todos1;
     assert forall k :: k in todos ==> AVersionIsMetOnAllServers(b, i, k, todos[k].vc) && AllVersionsInDepsAreMetOnAllServers(b, i, todos[k].deps);
 
@@ -155,6 +236,9 @@ lemma lemma_VersionsAfterPullDepsAreMetOnAllServers(
     assert res.1 == new_cache;
     assert AllVersionsInCCacheAreMetOnAllServers(b, i, res.1);
 }
+
+
+
 
 
 lemma {:axiom} lemma_MetaMapIsMetImpliesInsertedMataMapIsMet(
@@ -178,41 +262,7 @@ lemma {:axiom} lemma_MetaMapIsMetImpliesInsertedMataMapIsMet(
 
 // }
 
-lemma lemma_MetaIsMetImpliesMetasBeforeItAreMet(
-    b:Behavior<CMState>,
-    i:int,
-    meta:Meta,
-    metas:set<Meta>
-)
-    requires i > 0
-    requires IsValidBehaviorPrefix(b, i)
-    // requires forall j :: 0 <= j < i ==> CMNext(b[j], b[j+1])
-    requires CMNext(b[i-1], b[i])
-    requires MetaValid(meta)
-    requires AVersionIsMetOnAllServers(b, i, meta.key, meta.vc)
-    requires forall j :: 0 < j <= i ==> AllWriteDepsAreMet(b, j)
-    requires forall m :: m in metas ==> MetaValid(m) && (VCHappendsBefore(m.vc, meta.vc) || VCEq(m.vc, meta.vc))
-    ensures forall m :: m in metas ==> AVersionIsMetOnAllServers(b, i, m.key, m.vc)
-    ensures forall m :: m in metas ==> AllVersionsInDepsAreMetOnAllServers(b, i, m.deps)
-{
-    reveal_AllVersionsInDepsAreMetOnAllServers();
-    forall m | m in metas 
-        ensures AVersionIsMetOnAllServers(b, i, m.key, m.vc);
-        ensures AllVersionsInDepsAreMetOnAllServers(b, i, m.deps)
-    {
-        assert VCHappendsBefore(m.vc, meta.vc) || VCEq(m.vc, meta.vc);
-        lemma_MetaIsMetImpliesAllPreviousMetasAreMet(b, i, meta, m);
-        assert AVersionIsMetOnAllServers(b, i, m.key, m.vc);
-        assert i > 0;
-        assert IsValidBehaviorPrefix(b, i);
-        assert MetaValid(m);
-        assert AVersionIsMetOnAllServers(b, i, m.key, m.vc);
-        assert forall j :: 0 < j <= i ==> AllWriteDepsAreMet(b, j);
-        lemma_MetaIsMetImpliesItsDepsAreMet(b, i, m);
-        assert AllVersionsInDepsAreMetOnAllServers(b, i, m.deps);
-        assert AVersionIsMetOnAllServers(b, i, m.key, m.vc);
-    }
-}
+
 
 lemma {:axiom} lemma_FoldMetasPreservesDepsAreMet(
     b:Behavior<CMState>,
@@ -261,7 +311,114 @@ lemma {:axiom} lemma_FoldMetasPreservesDepsAreMet(
 //     assert AllVersionsInDepsAreMetOnAllServers(b, i, FoldMetaSet(meta, metas, domain).deps);
 // }
 
-function GetMetasOfAllDepsGlobalView(
+// function {:opaque} GetMetasOfAllDepsGlobalView(
+//     b:Behavior<CMState>,
+//     i:int,
+//     idx:int,
+//     icache:ICache,
+//     deps:Dependency,
+//     todos:map<Key, Meta>,
+//     domain:set<Key>
+// ) : (res:map<Key, Meta>)
+//     requires i > 0
+//     requires IsValidBehaviorPrefix(b, i)
+//     // requires forall j :: 0 <= j < i ==> CMNext(b[j], b[j+1])
+//     requires CMNext(b[i-1], b[i])
+//     requires forall k :: k in icache ==> k in Keys_domain && (forall m :: m in icache[k] ==> MetaValid(m) && m.key == k
+//                 && (forall kk :: kk in m.deps ==> kk in domain && kk in Keys_domain))
+//     requires DependencyValid(deps)
+//     requires forall k :: k in todos ==> MetaValid(todos[k]) && todos[k].key == k 
+//     requires forall k :: k in Keys_domain ==> k in icache // should we have this?
+//     requires forall k :: k in deps ==> k in domain 
+
+//     requires forall j :: 0 < j <= i ==> AllWriteDepsAreMet(b, j)
+//     requires forall j :: 0 <= j < i ==> ServerNextDoesNotDecreaseVersions(b[j], b[j+1])
+
+//     requires AllVersionsInDepsAreMetOnAllServers(b, i, deps)
+//     requires forall k :: k in todos ==> AVersionIsMetOnAllServers(b, i, k, todos[k].vc) && AllVersionsInDepsAreMetOnAllServers(b, i, todos[k].deps)
+
+//     ensures forall k :: k in res ==> MetaValid(res[k]) && res[k].key == k 
+//     ensures forall k :: k in res ==> AVersionIsMetOnAllServers(b, i, k, res[k].vc) && AllVersionsInDepsAreMetOnAllServers(b, i, res[k].deps)
+//     decreases |icache.Values|, |deps|
+// {
+//     reveal_AllVersionsInDepsAreMetOnAllServers();
+//     // reveal_AllVersionsInCCacheAreMetOnAllServers();
+    
+//     // assert forall k :: k in todos ==> AVersionIsMetOnAllServers(b, i, k, todos[k].vc); //&& AllVersionsInDepsAreMetOnAllServers(b, i, todos[k].deps);
+//     if |deps| == 0 then 
+//         todos
+//     else 
+//         var k :| k in deps;
+//         var new_deps := RemoveElt(deps, k);
+//         if k in todos && (VCHappendsBefore(deps[k], todos[k].vc) || VCEq(deps[k], todos[k].vc)) then 
+//             var res := GetMetasOfAllDepsGlobalView(b, i, idx, icache, new_deps, todos, domain);
+//             res
+//         else 
+//             var metas := set m | m in icache[k] && (VCHappendsBefore(m.vc, deps[k]) || VCEq(m.vc, deps[k]));
+//             if |metas| > 0 then
+//             // if exists m :: m in icache[k] && VCEq(m.vc, deps[k]) then 
+//                 var initial := EmptyMeta(k);
+//                 var merged := FoldMetaSet(initial, metas, domain);
+//                 var meta := merged.(vc := deps[k]);
+//                 // var m :| m in icache[k] && VCEq(m.vc, deps[k]);
+//                 // var meta := m;
+                
+//                 lemma_FoldMetaBounded(initial, metas, deps[k], domain);
+//                 assert (VCHappendsBefore(merged.vc, meta.vc) || VCEq(merged.vc, meta.vc));
+
+//                 var new_cache := icache[k:= icache[k] - metas];
+//                 assert icache[k] >= metas;
+//                 lemma_MapRemoveSubsetOfTheValOfKey(icache, k, metas);
+//                 assert |new_cache.Values| < |icache.Values|;
+
+//                 assert forall m :: m in metas ==> VCHappendsBefore(m.vc, meta.vc) || VCEq(m.vc, meta.vc);
+//                 assert forall m :: m in metas ==> m in icache[m.key];
+//                 assume AVersionIsMetOnAllServers(b, i, meta.key, meta.vc);
+//                 lemma_MetaIsMetImpliesMetasBeforeItAreMet(b, i, meta, metas);
+//                 assert forall m :: m in metas ==> AVersionIsMetOnAllServers(b, i, m.key, m.vc);
+//                 assert forall m :: m in metas ==> AllVersionsInDepsAreMetOnAllServers(b, i, m.deps);
+//                 // assume forall j :: 0 <= j < i ==> CMNext(b[j], b[j+1]);
+//                 // assert MetaValid(meta);
+//                 // assert forall j :: 0 < j <= i ==> AllWriteDepsAreMet(b, j);
+//                 // lemma_MetaIsMetImpliesItsDepsAreMet(b, i, meta);
+
+//                 assert MetaValid(initial);
+//                 assert forall kk :: kk in initial.deps ==> kk in domain;
+//                 assert AllVersionsInDepsAreMetOnAllServers(b, i, initial.deps);
+//                 lemma_FoldMetasPreservesDepsAreMet(b, i, initial, metas, domain);
+//                 assert AllVersionsInDepsAreMetOnAllServers(b, i, meta.deps);
+
+//                 var res := GetMetasOfAllDepsGlobalView(b, i, idx, new_cache, merged.deps, todos, domain);
+
+//                 assume forall k :: k in res ==> AVersionIsMetOnAllServers(b, i, k, res[k].vc) && AllVersionsInDepsAreMetOnAllServers(b, i, res[k].deps);
+//                 assume AVersionIsMetOnAllServers(b, i, k, meta.vc);
+
+//                 var todos' := AddMetaToMetaMap(res, meta);
+
+//                 assume AllVersionsInDepsAreMetOnAllServers(b, i, new_deps);
+//                 lemma_MetaMapIsMetImpliesInsertedMataMapIsMet(b, i, res, meta);
+//                 assume forall k :: k in todos' ==> AVersionIsMetOnAllServers(b, i, k, todos'[k].vc) && AllVersionsInDepsAreMetOnAllServers(b, i, todos'[k].deps);
+
+//                 var res' := GetMetasOfAllDepsGlobalView(b, i, idx, icache, new_deps, todos', domain);
+//                 res'
+//             else 
+//                 var initial := EmptyMeta(k);
+//                 var meta := initial.(vc:=deps[k]);
+
+//                 assume AllVersionsInDepsAreMetOnAllServers(b, i, deps);
+//                 assume forall k :: k in todos ==> AVersionIsMetOnAllServers(b, i, k, todos[k].vc) && AllVersionsInDepsAreMetOnAllServers(b, i, todos[k].deps);
+//                 assert AVersionIsMetOnAllServers(b, i, meta.key, meta.vc);
+//                 assert AllVersionsInDepsAreMetOnAllServers(b, i, meta.deps);
+                
+//                 var todos' := AddMetaToMetaMap(todos, meta);
+//                 lemma_MetaMapIsMetImpliesInsertedMataMapIsMet(b, i, todos, meta);
+//                 assert forall k :: k in todos' ==> AVersionIsMetOnAllServers(b, i, k, todos'[k].vc) && AllVersionsInDepsAreMetOnAllServers(b, i, todos'[k].deps);
+                
+//                 var res := GetMetasOfAllDepsGlobalView(b, i, idx, icache, new_deps, todos', domain);
+//                 res
+// }
+
+function {:opaque} GetMetasOfAllDepsGlobalView2(
     b:Behavior<CMState>,
     i:int,
     idx:int,
@@ -274,6 +431,10 @@ function GetMetasOfAllDepsGlobalView(
     requires IsValidBehaviorPrefix(b, i)
     // requires forall j :: 0 <= j < i ==> CMNext(b[j], b[j+1])
     requires CMNext(b[i-1], b[i])
+    requires 0 <= idx < Nodes
+    // requires icache == b[i].servers[idx].s.icache
+    requires forall k :: k in icache ==> forall m :: m in icache[k] ==> k in b[i].servers[idx].s.icache && m in b[i].servers[idx].s.icache[k]
+
     requires forall k :: k in icache ==> k in Keys_domain && (forall m :: m in icache[k] ==> MetaValid(m) && m.key == k
                 && (forall kk :: kk in m.deps ==> kk in domain && kk in Keys_domain))
     requires DependencyValid(deps)
@@ -282,6 +443,7 @@ function GetMetasOfAllDepsGlobalView(
     requires forall k :: k in deps ==> k in domain 
 
     requires forall j :: 0 < j <= i ==> AllWriteDepsAreMet(b, j)
+    requires forall j :: 0 <= j < i ==> ServerNextDoesNotDecreaseVersions(b[j], b[j+1])
 
     requires AllVersionsInDepsAreMetOnAllServers(b, i, deps)
     requires forall k :: k in todos ==> AVersionIsMetOnAllServers(b, i, k, todos[k].vc) && AllVersionsInDepsAreMetOnAllServers(b, i, todos[k].deps)
@@ -300,7 +462,7 @@ function GetMetasOfAllDepsGlobalView(
         var k :| k in deps;
         var new_deps := RemoveElt(deps, k);
         if k in todos && (VCHappendsBefore(deps[k], todos[k].vc) || VCEq(deps[k], todos[k].vc)) then 
-            var res := GetMetasOfAllDepsGlobalView(b, i, idx, icache, new_deps, todos, domain);
+            var res := GetMetasOfAllDepsGlobalView2(b, i, idx, icache, new_deps, todos, domain);
             res
         else 
             var metas := set m | m in icache[k] && (VCHappendsBefore(m.vc, deps[k]) || VCEq(m.vc, deps[k]));
@@ -321,8 +483,10 @@ function GetMetasOfAllDepsGlobalView(
                 assert |new_cache.Values| < |icache.Values|;
 
                 assert forall m :: m in metas ==> VCHappendsBefore(m.vc, meta.vc) || VCEq(m.vc, meta.vc);
+                assert forall m :: m in metas ==> m in icache[m.key];
+                assert forall m :: m in metas ==> AVersionOfAKeyIsMet(b[i].servers[idx].s.icache, b[i].servers[idx].s.ccache, m.key, m.vc);
                 assume AVersionIsMetOnAllServers(b, i, meta.key, meta.vc);
-                lemma_MetaIsMetImpliesMetasBeforeItAreMet(b, i, meta, metas);
+                lemma_MetaIsMetImpliesMetasBeforeItAreMet2(b, i, idx, meta, metas);
                 assert forall m :: m in metas ==> AVersionIsMetOnAllServers(b, i, m.key, m.vc);
                 assert forall m :: m in metas ==> AllVersionsInDepsAreMetOnAllServers(b, i, m.deps);
                 // assume forall j :: 0 <= j < i ==> CMNext(b[j], b[j+1]);
@@ -336,7 +500,7 @@ function GetMetasOfAllDepsGlobalView(
                 lemma_FoldMetasPreservesDepsAreMet(b, i, initial, metas, domain);
                 assert AllVersionsInDepsAreMetOnAllServers(b, i, meta.deps);
 
-                var res := GetMetasOfAllDepsGlobalView(b, i, idx, new_cache, merged.deps, todos, domain);
+                var res := GetMetasOfAllDepsGlobalView2(b, i, idx, new_cache, merged.deps, todos, domain);
 
                 assume forall k :: k in res ==> AVersionIsMetOnAllServers(b, i, k, res[k].vc) && AllVersionsInDepsAreMetOnAllServers(b, i, res[k].deps);
                 assume AVersionIsMetOnAllServers(b, i, k, meta.vc);
@@ -347,7 +511,7 @@ function GetMetasOfAllDepsGlobalView(
                 lemma_MetaMapIsMetImpliesInsertedMataMapIsMet(b, i, res, meta);
                 assume forall k :: k in todos' ==> AVersionIsMetOnAllServers(b, i, k, todos'[k].vc) && AllVersionsInDepsAreMetOnAllServers(b, i, todos'[k].deps);
 
-                var res' := GetMetasOfAllDepsGlobalView(b, i, idx, icache, new_deps, todos', domain);
+                var res' := GetMetasOfAllDepsGlobalView2(b, i, idx, icache, new_deps, todos', domain);
                 res'
             else 
                 var initial := EmptyMeta(k);
@@ -362,11 +526,10 @@ function GetMetasOfAllDepsGlobalView(
                 lemma_MetaMapIsMetImpliesInsertedMataMapIsMet(b, i, todos, meta);
                 assert forall k :: k in todos' ==> AVersionIsMetOnAllServers(b, i, k, todos'[k].vc) && AllVersionsInDepsAreMetOnAllServers(b, i, todos'[k].deps);
                 
-                var res := GetMetasOfAllDepsGlobalView(b, i, idx, icache, new_deps, todos', domain);
+                var res := GetMetasOfAllDepsGlobalView2(b, i, idx, icache, new_deps, todos', domain);
                 res
 }
 
-
 // function GetMetasOfAllDepsGlobalView(
 //     b:Behavior<CMState>,
 //     i:int,
@@ -536,7 +699,40 @@ function GetMetasOfAllDepsGlobalView(
 // }
 
 
-lemma {:axiom} lemma_GetMetasOfAllDepsGlobalViewEqualsToGetMetasOfAllDeps
+// lemma {:axiom} lemma_GetMetasOfAllDepsGlobalViewEqualsToGetMetasOfAllDeps
+// (
+//     b:Behavior<CMState>,
+//     i:int,
+//     idx:int,
+//     icache:ICache,
+//     deps:Dependency,
+//     todos:map<Key, Meta>,
+//     domain:set<Key>
+// )
+//     requires i > 0
+//     requires IsValidBehaviorPrefix(b, i)
+//     requires CMNext(b[i-1], b[i]);
+//     requires forall k :: k in icache ==> k in Keys_domain && (forall m :: m in icache[k] ==> MetaValid(m) && m.key == k
+//                 && (forall kk :: kk in m.deps ==> kk in domain && kk in Keys_domain))
+//     requires DependencyValid(deps)
+//     requires forall k :: k in todos ==> MetaValid(todos[k]) && todos[k].key == k 
+//     requires forall k :: k in Keys_domain ==> k in icache // should we have this?
+//     requires forall k :: k in deps ==> k in domain 
+
+//     requires forall k :: k in todos ==> forall kk :: kk in todos[k].deps ==> 
+//                         VCHappendsBefore(todos[k].deps[kk], todos[k].vc) || VCEq(todos[k].deps[kk], todos[k].vc)
+//     requires CausalCut(todos)
+
+//     requires forall j :: 0 < j <= i ==> AllWriteDepsAreMet(b, j)
+//     requires forall j :: 0 <= j < i ==> ServerNextDoesNotDecreaseVersions(b[j], b[j+1])
+//     requires AllVersionsInDepsAreMetOnAllServers(b, i, deps)
+//     requires forall k :: k in todos ==> AVersionIsMetOnAllServers(b, i, k, todos[k].vc) && AllVersionsInDepsAreMetOnAllServers(b, i, todos[k].deps)
+//     ensures 
+//             var res1 := GetMetasOfAllDepsGlobalView(b, i, idx, icache, deps, todos, domain);
+//             var res2 := GetMetasOfAllDeps(icache, deps, todos, domain);
+//             res1 == res2
+
+lemma {:axiom} lemma_GetMetasOfAllDepsGlobalViewEqualsToGetMetasOfAllDeps2
 (
     b:Behavior<CMState>,
     i:int,
@@ -548,7 +744,10 @@ lemma {:axiom} lemma_GetMetasOfAllDepsGlobalViewEqualsToGetMetasOfAllDeps
 )
     requires i > 0
     requires IsValidBehaviorPrefix(b, i)
-    requires CMNext(b[i-1], b[i]);
+    requires CMNext(b[i-1], b[i])
+    requires 0 <= idx < Nodes
+    requires icache == b[i].servers[idx].s.icache
+
     requires forall k :: k in icache ==> k in Keys_domain && (forall m :: m in icache[k] ==> MetaValid(m) && m.key == k
                 && (forall kk :: kk in m.deps ==> kk in domain && kk in Keys_domain))
     requires DependencyValid(deps)
@@ -561,10 +760,11 @@ lemma {:axiom} lemma_GetMetasOfAllDepsGlobalViewEqualsToGetMetasOfAllDeps
     requires CausalCut(todos)
 
     requires forall j :: 0 < j <= i ==> AllWriteDepsAreMet(b, j)
+    requires forall j :: 0 <= j < i ==> ServerNextDoesNotDecreaseVersions(b[j], b[j+1])
     requires AllVersionsInDepsAreMetOnAllServers(b, i, deps)
     requires forall k :: k in todos ==> AVersionIsMetOnAllServers(b, i, k, todos[k].vc) && AllVersionsInDepsAreMetOnAllServers(b, i, todos[k].deps)
     ensures 
-            var res1 := GetMetasOfAllDepsGlobalView(b, i, idx, icache, deps, todos, domain);
+            var res1 := GetMetasOfAllDepsGlobalView2(b, i, idx, icache, deps, todos, domain);
             var res2 := GetMetasOfAllDeps(icache, deps, todos, domain);
             res1 == res2
 }
