DistributedSystems/VerifiedDS/src/Dafny/Distributed/Protocol/CausalMesh/proof/clients_are_met.dfy
@@ -26,6 +26,7 @@ import opened CausalMesh_Proof_DepsAreMet_i
 import opened CausalMesh_Proof_ReadReplyIsMet_i
 import opened CausalMesh_Proof_Propagation_i
 import opened CausalMesh_Proof_PropagationLemma2_i
+import opened CausalMesh_Proof_AllwaysMet_i
 import opened Collections__Seqs_s
 import opened Collections__Maps_i
 import opened Collections__Maps2_s
