DistributedSystems/VerifiedDS/src/Dafny/Distributed/Protocol/CausalMesh/proof/meta_is_met.dfy
@@ -3,6 +3,8 @@ include "../distributed_system.dfy"
 include "packet_sending.dfy"
 include "properties.dfy"
 include "propagation.dfy"
+include "propagation_lemma3.dfy"
+include "always_met.dfy"
 include "../../../Common/Collections/Seqs.s.dfy"
 
 module CausalMesh_Proof_MetaIsMet_i {
@@ -17,31 +19,149 @@ import opened Temporal__Temporal_s
 import opened CausalMesh_proof_Assumptions_i
 import opened CausalMesh_Proof_Constants_i
 import opened CausalMesh_Proof_PropagationLemma_i
+import opened CausalMesh_Proof_PropagationLemma3_i
 import opened CausalMesh_Proof_Propagation_i
 import opened CausalMesh_Proof_PacketSending_i
 import opened CausalMesh_Proof_Properties_i
+import opened CausalMesh_Proof_AllwaysMet_i
 // import opened CausalMesh_Proof_MessageReadReply_i
 import opened Collections__Seqs_s
 import opened Collections__Maps_i
 import opened Collections__Maps2_s
 
-lemma lemma_MetaIsMetImpliesItsDepsAreMet(
+// lemma lemma_MetaIsMetImpliesItsDepsAreMet(
+//     b:Behavior<CMState>,
+//     i:int,
+//     meta:Meta
+// )
+//     requires 0 < i 
+//     requires IsValidBehaviorPrefix(b, i)
+//     // requires forall j :: 0 <= j < i ==> CMNext(b[j], b[j+1])
+//     requires MetaValid(meta)
+//     requires AVersionIsMetOnAllServers(b, i, meta.key, meta.vc)
+//     requires forall j :: 0 < j <= i ==> AllWriteDepsAreMet(b, j)
+//     requires forall j :: 0 <= j < i ==> ServerNextDoesNotDecreaseVersions(b[j], b[j+1])
+//     ensures AllVersionsInDepsAreMetOnAllServers(b, i, meta.deps)
+// {
+//     if i == 0 {
+//         return;
+//     }
+
+//     if i == 1 {
+//         lemma_BehaviorValidImpliesOneStepValid(b, i);
+//         assert CMNext(b[i-1], b[i]);
+//         lemma_MetaIsMetImpliesItsDepsAreMetForIndexOne(b, i, meta);
+//         // reveal_AllVersionsInDepsAreMetOnAllServers();
+//         assert AllVersionsInDepsAreMetOnAllServers(b, i, meta.deps);
+//         return;
+//     }
+
+//     assert 0 < i - 1;
+
+//     lemma_ConstantsAllConsistent(b, i-1);
+//     lemma_ConstantsAllConsistent(b, i);
+
+//     lemma_BehaviorValidImpliesOneStepValid(b, i);
+
+//     if AVersionIsMetOnAllServers(b, i-1, meta.key, meta.vc)
+//     {
+//         lemma_MetaIsMetImpliesItsDepsAreMet(b, i-1, meta);
+//         assume ServerNextDoesNotDecreaseVersions(b[i-1], b[i]);
+//         assert i > 1;
+//         assert IsValidBehaviorPrefix(b, i);
+//         assert CMNext(b[i-1], b[i]);
+//         assert DependencyValid(meta.deps);
+//         assume AllVersionsInDepsAreMetOnAllServers(b, i-1, meta.deps);
+//         lemma_AllVersionsInDepsAreMetOnAllServersWillAlwaysMet(b, i, meta.deps);
+//         return;
+//     }
+
+//     // var ios := lemma_ActionThatChangesServerIsThatServersAction(b, i, )
+    
+//     // how to find the node that is the tail of propagation of meta?
+
+//     var ios:seq<CMIo>;
+//     var idx :| 0 <= idx < Nodes;
+
+//     assert CMNext(b[i-1], b[i]);
+//     assert 0 < i; 
+//     assert IsValidBehaviorPrefix(b, i);
+//     assert MetaValid(meta);
+//     assert 0 <= idx < Nodes;
+
+//     lemma_IosIsPropagationTail(b, i, idx, ios, meta);
+
+//     assert ReceivePropagate(b[i-1].servers[idx].s, b[i].servers[idx].s, ios[0].r, ExtractSentPacketsFromIos(ios));
+
+//     var p_pro := ios[0].r;
+//     assert p_pro.dst == idx;
+
+//     lemma_PropagationAtTail2(b, i, idx, p_pro, ios);
+//     assert AllVersionsInDepsAreMetOnAllServers(b, i, p_pro.msg.meta.deps);
+//     assert AllVersionsInDepsAreMetOnAllServers(b, i, meta.deps);
+// }
+
+lemma lemma_MetaIsMetImpliesItsDepsAreMet2(
     b:Behavior<CMState>,
     i:int,
+    idx:int,
     meta:Meta
 )
     requires 0 < i 
     requires IsValidBehaviorPrefix(b, i)
-    // requires forall j :: 0 <= j < i ==> CMNext(b[j], b[j+1])
+    requires CMNext(b[i-1], b[i])
+    requires 0 <= idx < Nodes
     requires MetaValid(meta)
+    requires AVersionOfAKeyIsMet(b[i].servers[idx].s.icache, b[i].servers[idx].s.ccache, meta.key, meta.vc)
+    // requires meta in b[i].servers[idx].s.icache[meta.key]
+    // requires meta != EmptyMeta(meta.key)
+    // requires forall j :: 0 <= j < i ==> CMNext(b[j], b[j+1])
+    
     requires AVersionIsMetOnAllServers(b, i, meta.key, meta.vc)
     requires forall j :: 0 < j <= i ==> AllWriteDepsAreMet(b, j)
+    requires forall j :: 0 <= j < i ==> ServerNextDoesNotDecreaseVersions(b[j], b[j+1])
     ensures AllVersionsInDepsAreMetOnAllServers(b, i, meta.deps)
 {
-     if i <= 1 {
+    if i == 0 {
+        return;
+    }
+
+    if i == 1 {
         lemma_BehaviorValidImpliesOneStepValid(b, i);
         assert CMNext(b[i-1], b[i]);
-        lemma_MetaIsMetImpliesItsDepsAreMetForIndexOne(b, i, meta);
+        lemma_MetaIsMetImpliesItsDepsAreMetForIndexOne2(b, i);
+        // reveal_AllVersionsInDepsAreMetOnAllServers();
+        // assert AllVersionsInDepsAreMetOnAllServers(b, i, meta.deps);
+        assert b[i].servers[idx].s.icache == InitICache();
+        assert b[i].servers[idx].s.ccache == InitCCache();
+        if meta != EmptyMeta(meta.key){
+            if VCHappendsBefore(EmptyMeta(meta.key).vc, meta.vc) {
+                assert meta !in b[i].servers[idx].s.icache[meta.key];
+                assert !(VCHappendsBefore(meta.vc, b[i].servers[idx].s.ccache[meta.key].vc) || VCEq(meta.vc, b[i].servers[idx].s.ccache[meta.key].vc));
+                var m := FoldMetaSet2(b[i].servers[idx].s.ccache[meta.key], b[i].servers[idx].s.icache[meta.key]);
+                assert b[i].servers[idx].s.ccache[meta.key] == EmptyMeta(meta.key);
+                assert forall m :: m in b[i].servers[idx].s.icache[meta.key] ==> m == EmptyMeta(meta.key);
+                lemma_FoldEmptyMetasResultInEmptyMeta(b[i].servers[idx].s.ccache[meta.key], b[i].servers[idx].s.icache[meta.key]);
+                assert m == EmptyMeta(meta.key);
+                assert !AVersionOfAKeyIsMet(b[i].servers[idx].s.icache, b[i].servers[idx].s.ccache, meta.key, meta.vc);
+                assert false;
+            } else {
+                lemma_MetaWithNonEmptyDepsImpliesTheVCLargerThanZero(meta);
+                assert meta !in b[i].servers[idx].s.icache[meta.key];
+                assert !(VCHappendsBefore(meta.vc, b[i].servers[idx].s.ccache[meta.key].vc) || VCEq(meta.vc, b[i].servers[idx].s.ccache[meta.key].vc));
+                var m := FoldMetaSet2(b[i].servers[idx].s.ccache[meta.key], b[i].servers[idx].s.icache[meta.key]);
+                assert b[i].servers[idx].s.ccache[meta.key] == EmptyMeta(meta.key);
+                assert forall m :: m in b[i].servers[idx].s.icache[meta.key] ==> m == EmptyMeta(meta.key);
+                lemma_FoldEmptyMetasResultInEmptyMeta(b[i].servers[idx].s.ccache[meta.key], b[i].servers[idx].s.icache[meta.key]);
+                assert m == EmptyMeta(meta.key);
+                assert !AVersionOfAKeyIsMet(b[i].servers[idx].s.icache, b[i].servers[idx].s.ccache, meta.key, meta.vc);
+                assert false;
+            }
+        } 
+        else {
+            reveal_AllVersionsInDepsAreMetOnAllServers();
+            assert AllVersionsInDepsAreMetOnAllServers(b, i, meta.deps);
+        }
         return;
     }
 
@@ -54,8 +174,15 @@ lemma lemma_MetaIsMetImpliesItsDepsAreMet(
 
     if AVersionIsMetOnAllServers(b, i-1, meta.key, meta.vc)
     {
-        lemma_MetaIsMetImpliesItsDepsAreMet(b, i-1, meta);
-        lemma_DepsAreMetAreTransitive(b, i, meta);
+        // assume meta in b[i-1].servers[idx].s.icache[meta.key];
+        lemma_MetaIsMetImpliesItsDepsAreMet2(b, i-1, idx, meta);
+        assume ServerNextDoesNotDecreaseVersions(b[i-1], b[i]);
+        assert i > 1;
+        assert IsValidBehaviorPrefix(b, i);
+        assert CMNext(b[i-1], b[i]);
+        assert DependencyValid(meta.deps);
+        assume AllVersionsInDepsAreMetOnAllServers(b, i-1, meta.deps);
+        lemma_AllVersionsInDepsAreMetOnAllServersWillAlwaysMet(b, i, meta.deps);
         return;
     }
 
@@ -84,32 +211,37 @@ lemma lemma_MetaIsMetImpliesItsDepsAreMet(
     assert AllVersionsInDepsAreMetOnAllServers(b, i, meta.deps);
 }
 
-lemma {:axiom} lemma_MetaIsMetImpliesItsDepsAreMetForIndexOne(
+// lemma {:axiom} lemma_MetaIsMetImpliesItsDepsAreMetForIndexOne(
+//     b:Behavior<CMState>,
+//     i:int
+//     ,
+//     meta:Meta
+// )
+//     requires i == 1 
+//     requires IsValidBehaviorPrefix(b, i)
+//     requires CMNext(b[i-1], b[i])
+//     requires MetaValid(meta)
+//     ensures !exists p :: p in b[i].environment.sentPackets && p.msg.Message_Propagation?
+//     ensures AllVersionsInDepsAreMetOnAllServers(b, i, meta.deps)
+// // {
+// //     assert CMNext(b[i-1], b[i]);
+// // }
+
+lemma lemma_MetaIsMetImpliesItsDepsAreMetForIndexOne2(
     b:Behavior<CMState>,
-    i:int,
-    meta:Meta
+    i:int
 )
     requires i == 1 
     requires IsValidBehaviorPrefix(b, i)
     requires CMNext(b[i-1], b[i])
-    requires MetaValid(meta)
+    // requires 0 <= idx < Nodes
+    // requires meta in b[i].servers[idx].s.icache[meta.key]
+    // requires MetaValid(meta)
     ensures !exists p :: p in b[i].environment.sentPackets && p.msg.Message_Propagation?
-    ensures AllVersionsInDepsAreMetOnAllServers(b, i, meta.deps)
-
-lemma {:axiom} lemma_DepsAreMetAreTransitive(
-    b:Behavior<CMState>,
-    i:int,
-    meta:Meta
-)
-    requires i > 1 
-    requires IsValidBehaviorPrefix(b, i)
-    requires CMNext(b[i-1], b[i])
-    requires MetaValid(meta)
-    requires AllVersionsInDepsAreMetOnAllServers(b, i-1, meta.deps)
-    ensures AllVersionsInDepsAreMetOnAllServers(b, i, meta.deps)
-// {
-
-// }
+    // ensures AllVersionsInDepsAreMetOnAllServers(b, i, meta.deps)
+{
+    assert CMNext(b[i-1], b[i]);
+}
 
 lemma {:axiom} lemma_IosIsPropagationTail(
     b:Behavior<CMState>,
