DistributedSystems/VerifiedDS/src/Dafny/Distributed/Protocol/CausalMesh/proof/propagation.dfy
@@ -2,7 +2,7 @@ include "../distributed_system.dfy"
 // include "causalcut.dfy"
 include "packet_sending.dfy"
 include "properties.dfy"
-include "propagation_lemma2.dfy"
+include "propagation_lemma3.dfy"
 include "../../../Common/Collections/Seqs.s.dfy"
 
 module CausalMesh_Proof_Propagation_i {
@@ -17,6 +17,7 @@ import opened Temporal__Temporal_s
 import opened CausalMesh_proof_Assumptions_i
 import opened CausalMesh_Proof_Constants_i
 import opened CausalMesh_Proof_PropagationLemma2_i
+import opened CausalMesh_Proof_PropagationLemma3_i
 import opened CausalMesh_Proof_PacketSending_i
 import opened CausalMesh_Proof_Properties_i
 // import opened CausalMesh_Proof_MessageReadReply_i
@@ -85,7 +86,8 @@ lemma lemma_PropagationAtTail(
     assert NodesAreNext(s.id, p.msg.start);
     assert p.dst == s.id;
     lemma_NodesFormACircle(p.msg.start, p.dst, nodes);
-    assert forall j :: 0 <= j < Nodes ==> j in nodes;
+    // assert forall j :: 0 <= j < Nodes ==> j in nodes;
+    assert NodesAreComplete(nodes);
 
     var new_deps := p.msg.meta.deps;
     var (new_icache, new_ccache) := PullDeps2(s.icache, s.ccache, new_deps);
@@ -116,104 +118,104 @@ lemma lemma_PropagationAtTail(
     // assert AVersionIsMetOnAllServers(b, i, p.msg.key, p.msg.meta.vc);
 }
 
-lemma lemma_PropagationAtTail2(
-    b:Behavior<CMState>,
-    i:int,
-    idx:int,
-    p:Packet,
-    ios:seq<CMIo>
-)
-    requires 0 < i 
-    requires IsValidBehaviorPrefix(b, i)
-    // requires forall j :: 0 <= j < i ==> CMNext(b[j], b[j+1])
-    requires CMNext(b[i-1], b[i])
-    requires forall j :: 0 < j <= i ==> AllWriteDepsAreMet(b, j)
-    requires 0 <= idx < Nodes
-    requires |ios| > 0
-    requires ios[0].LIoOpReceive?
-    requires p.msg.Message_Propagation?
-    requires p in b[i-1].environment.sentPackets
-    requires p.dst == idx
-    requires idx == b[i-1].servers[idx].s.id
-    requires ios[0].r == p
-    requires PacketValid(p)
-    requires p.msg.start == b[i-1].servers[idx].s.next
-    requires p.msg.round == 2
-    requires ReceivePropagate(b[i-1].servers[idx].s, b[i].servers[idx].s, p, ExtractSentPacketsFromIos(ios))
-    ensures AllVersionsInDepsAreMetOnAllServers(b, i, p.msg.meta.deps)
-{
-    var p := ios[0].r;
-    var s := b[i-1].servers[idx].s;
-    var s' := b[i].servers[idx].s;
+// lemma lemma_PropagationAtTail2(
+//     b:Behavior<CMState>,
+//     i:int,
+//     idx:int,
+//     p:Packet,
+//     ios:seq<CMIo>
+// )
+//     requires 0 < i 
+//     requires IsValidBehaviorPrefix(b, i)
+//     // requires forall j :: 0 <= j < i ==> CMNext(b[j], b[j+1])
+//     requires CMNext(b[i-1], b[i])
+//     requires forall j :: 0 < j <= i ==> AllWriteDepsAreMet(b, j)
+//     requires 0 <= idx < Nodes
+//     requires |ios| > 0
+//     requires ios[0].LIoOpReceive?
+//     requires p.msg.Message_Propagation?
+//     requires p in b[i-1].environment.sentPackets
+//     requires p.dst == idx
+//     requires idx == b[i-1].servers[idx].s.id
+//     requires ios[0].r == p
+//     requires PacketValid(p)
+//     requires p.msg.start == b[i-1].servers[idx].s.next
+//     requires p.msg.round == 2
+//     requires ReceivePropagate(b[i-1].servers[idx].s, b[i].servers[idx].s, p, ExtractSentPacketsFromIos(ios))
+//     ensures AllVersionsInDepsAreMetOnAllServers(b, i, p.msg.meta.deps)
+// {
+//     var p := ios[0].r;
+//     var s := b[i-1].servers[idx].s;
+//     var s' := b[i].servers[idx].s;
 
-    assert p.msg.start == s.next;
+//     assert p.msg.start == s.next;
 
-    assert 0 <= i - 1;
-    assert IsValidBehaviorPrefix(b, i-1);
-    assert forall j :: 0 <= j < i-1 ==> CMNext(b[j], b[j+1]);
-    // assert CMNext(b[i-2], b[i-1]);
-    assert CMNext(b[i-1], b[i]);
-    // assert CMNextCommon(b[i-1], b[i]);
-    assert forall j :: 0 <= j < Nodes ==> ServerValid(b[i-1].servers[j].s);
-    assert p.msg.Message_Propagation?;
-    assert CMInit(b[0]);
-    assert |b[i-1].servers| == Nodes;
-    assert p in b[i-1].environment.sentPackets;
-    assert PacketValid(p);
+//     assert 0 <= i - 1;
+//     assert IsValidBehaviorPrefix(b, i-1);
+//     assert forall j :: 0 <= j < i-1 ==> CMNext(b[j], b[j+1]);
+//     // assert CMNext(b[i-2], b[i-1]);
+//     assert CMNext(b[i-1], b[i]);
+//     // assert CMNextCommon(b[i-1], b[i]);
+//     assert forall j :: 0 <= j < Nodes ==> ServerValid(b[i-1].servers[j].s);
+//     assert p.msg.Message_Propagation?;
+//     assert CMInit(b[0]);
+//     assert |b[i-1].servers| == Nodes;
+//     assert p in b[i-1].environment.sentPackets;
+//     assert PacketValid(p);
 
-    assert p.dst == idx;
-    assert idx == s.id;
+//     assert p.dst == idx;
+//     assert idx == s.id;
 
-    var nodes := lemma_Propagation2(b, i-1, p);
-    assert |nodes| > 1;
-    assert nodes[0] == p.msg.start;
-    assert nodes[|nodes|-2] == p.src;
-    assert nodes[|nodes|-1] == p.dst;
-    assert forall j :: 0 <= j < |nodes| ==> 0 <= nodes[j] < Nodes;
-    assert forall j :: 0 <= j < |nodes| - 1 ==> NodesAreNext(nodes[j], nodes[j+1]);
-    assert forall j :: 0 <= j < |nodes| - 1 ==> AVersionOfAKeyIsMet(b[i-1].servers[nodes[j]].s.icache, b[i-1].servers[nodes[j]].s.ccache, p.msg.key, p.msg.meta.vc);
-    assert forall j :: 0 <= j < |nodes| - 1 ==> DepsIsMet(b[i-1].servers[nodes[j]].s.icache, b[i-1].servers[nodes[j]].s.ccache, p.msg.meta.deps);
+//     var nodes := lemma_Propagation2(b, i-1, p);
+//     assert |nodes| > 1;
+//     assert nodes[0] == p.msg.start;
+//     assert nodes[|nodes|-2] == p.src;
+//     assert nodes[|nodes|-1] == p.dst;
+//     assert forall j :: 0 <= j < |nodes| ==> 0 <= nodes[j] < Nodes;
+//     assert forall j :: 0 <= j < |nodes| - 1 ==> NodesAreNext(nodes[j], nodes[j+1]);
+//     assert forall j :: 0 <= j < |nodes| - 1 ==> AVersionOfAKeyIsMet(b[i-1].servers[nodes[j]].s.icache, b[i-1].servers[nodes[j]].s.ccache, p.msg.key, p.msg.meta.vc);
+//     assert forall j :: 0 <= j < |nodes| - 1 ==> DepsIsMet(b[i-1].servers[nodes[j]].s.icache, b[i-1].servers[nodes[j]].s.ccache, p.msg.meta.deps);
 
-    lemma_ServerNextSatisfyNodesAreNext(s.id, s.next);
-    assert NodesAreNext(s.id, p.msg.start);
-    assert p.dst == s.id;
-    lemma_NodesFormACircle(p.msg.start, p.dst, nodes);
-    assert forall j :: 0 <= j < Nodes ==> j in nodes;
+//     lemma_ServerNextSatisfyNodesAreNext(s.id, s.next);
+//     assert NodesAreNext(s.id, p.msg.start);
+//     assert p.dst == s.id;
+//     lemma_NodesFormACircle(p.msg.start, p.dst, nodes);
+//     assert forall j :: 0 <= j < Nodes ==> j in nodes;
 
-    var new_deps := p.msg.meta.deps;
-    var (new_icache, new_ccache) := PullDeps2(s.icache, s.ccache, new_deps);
-    // var merged_meta := MetaMerge(new_ccache[p.msg.key], p.msg.meta);
-    // assert VCHappendsBefore(p.msg.meta.vc, merged_meta.vc) || VCEq(p.msg.meta.vc, merged_meta.vc);
+//     var new_deps := p.msg.meta.deps;
+//     var (new_icache, new_ccache) := PullDeps2(s.icache, s.ccache, new_deps);
+//     // var merged_meta := MetaMerge(new_ccache[p.msg.key], p.msg.meta);
+//     // assert VCHappendsBefore(p.msg.meta.vc, merged_meta.vc) || VCEq(p.msg.meta.vc, merged_meta.vc);
 
-    var new_ccache' := InsertIntoCCache(new_ccache, p.msg.meta);
-    assert VCHappendsBefore(p.msg.meta.vc, new_ccache'[p.msg.key].vc) || VCEq(p.msg.meta.vc, new_ccache'[p.msg.key].vc);
-    // reveal_DepsIsMet();
-    lemma_DepsIsMet(b[i].servers[idx].s.icache, b[i].servers[idx].s.ccache, p.msg.meta.deps); // this could be proved, but may timeout
+//     var new_ccache' := InsertIntoCCache(new_ccache, p.msg.meta);
+//     assert VCHappendsBefore(p.msg.meta.vc, new_ccache'[p.msg.key].vc) || VCEq(p.msg.meta.vc, new_ccache'[p.msg.key].vc);
+//     // reveal_DepsIsMet();
+//     lemma_DepsIsMet(b[i].servers[idx].s.icache, b[i].servers[idx].s.ccache, p.msg.meta.deps); // this could be proved, but may timeout
     
-    lemma_AVersionOfAKeyIsMetIsTransitive(b, i, p.msg.key, p.msg.meta.vc, p.msg.meta.deps, nodes);
-    // assert forall j :: 0 <= j < |nodes| - 1 ==> AVersionOfAKeyIsMet(b[i].servers[nodes[j]].s.icache, b[i].servers[nodes[j]].s.ccache, p.msg.key, p.msg.meta.vc);
-    // assert forall j :: 0 <= j < |nodes| - 1 ==> DepsIsMet(b[i].servers[nodes[j]].s.icache, b[i].servers[nodes[j]].s.ccache, p.msg.meta.deps);
-    // assert forall j :: 0 <= j < |nodes| - 1 ==> AVersionOfAKeyIsMet(b[i].servers[nodes[j]].s.icache, b[i].servers[nodes[j]].s.ccache, p.msg.key, p.msg.meta.vc);
-    assert nodes[|nodes|-1] == idx;
+//     lemma_AVersionOfAKeyIsMetIsTransitive(b, i, p.msg.key, p.msg.meta.vc, p.msg.meta.deps, nodes);
+//     // assert forall j :: 0 <= j < |nodes| - 1 ==> AVersionOfAKeyIsMet(b[i].servers[nodes[j]].s.icache, b[i].servers[nodes[j]].s.ccache, p.msg.key, p.msg.meta.vc);
+//     // assert forall j :: 0 <= j < |nodes| - 1 ==> DepsIsMet(b[i].servers[nodes[j]].s.icache, b[i].servers[nodes[j]].s.ccache, p.msg.meta.deps);
+//     // assert forall j :: 0 <= j < |nodes| - 1 ==> AVersionOfAKeyIsMet(b[i].servers[nodes[j]].s.icache, b[i].servers[nodes[j]].s.ccache, p.msg.key, p.msg.meta.vc);
+//     assert nodes[|nodes|-1] == idx;
     
-    lemma_DepsIsMetForNodes(b, i, nodes, p.msg.meta.deps);
+//     lemma_DepsIsMetForNodes(b, i, nodes, p.msg.meta.deps);
 
-    assert |b[i].servers| == Nodes;
-    assert forall j :: 0 <= j < Nodes ==> ServerValid(b[i].servers[j].s);
-    assert |nodes| > 1;
-    assert forall j :: 0 <= j < |nodes| ==> 0 <= nodes[j] < Nodes;
-    // lemma_Nodes(nodes);
-    // assert forall j :: 0 <= j < Nodes ==> j in nodes;
-    lemma_DepsIsMetForAllNodes(b, i, nodes, p.msg.meta.deps);
-    assert AllVersionsInDepsAreMetOnAllServers(b, i, p.msg.meta.deps);
-}
+//     assert |b[i].servers| == Nodes;
+//     assert forall j :: 0 <= j < Nodes ==> ServerValid(b[i].servers[j].s);
+//     assert |nodes| > 1;
+//     assert forall j :: 0 <= j < |nodes| ==> 0 <= nodes[j] < Nodes;
+//     // lemma_Nodes(nodes);
+//     // assert forall j :: 0 <= j < Nodes ==> j in nodes;
+//     lemma_DepsIsMetForAllNodes(b, i, nodes, p.msg.meta.deps);
+//     assert AllVersionsInDepsAreMetOnAllServers(b, i, p.msg.meta.deps);
+// }
 
 // lemma {:axiom} lemma_Nodes(nodes:seq<int>)
 //     ensures forall j :: 0 <= j < Nodes ==> j in nodes
 
 // this one can be proved, but the last requires is not passed at the end of lemma_PropagationAtTail
 // but this requires is ture, beacuse it can pass at the middle of lemma_PropagationAtTail
-lemma {:axiom} lemma_AVersionOfAKeyIsMetForAllNodes(
+lemma lemma_AVersionOfAKeyIsMetForAllNodes(
     b:Behavior<CMState>,
     i:int,
     nodes:seq<int>,
@@ -231,45 +233,47 @@ lemma {:axiom} lemma_AVersionOfAKeyIsMetForAllNodes(
     requires forall j :: 0 <= j < |nodes| ==> 0 <= nodes[j] < Nodes 
     requires forall j :: 0 <= j < |nodes| ==> AVersionOfAKeyIsMet(b[i].servers[nodes[j]].s.icache, b[i].servers[nodes[j]].s.ccache, key, vc)
     // requires forall j :: 0 <= j < Nodes ==> j in nodes
+    requires NodesAreComplete(nodes)
     ensures AVersionIsMetOnAllServers(b, i, key, vc)
-// {
-//     // assume forall s :: s in b[i].servers ==> s.s.id in nodes;
-//     assert forall n :: n in nodes ==> AVersionOfAKeyIsMet(b[i].servers[n].s.icache, b[i].servers[n].s.ccache, key, vc);
-//     // assert forall s :: s in b[i].servers ==> AVersionOfAKeyIsMet(s.s.icache, s.s.ccache, key, vc);
-//     assert |b[i].servers| == Nodes;
-//     // assume |nodes| == Nodes;
-//     assert forall j :: 0 <= j < |b[i].servers| ==> j in nodes;
-//     assert forall j :: 0 <= j < |b[i].servers| ==> AVersionOfAKeyIsMet(b[i].servers[j].s.icache, b[i].servers[j].s.ccache, key, vc);
-// }
+{
+    reveal_NodesAreComplete();
+    // assume forall s :: s in b[i].servers ==> s.s.id in nodes;
+    assert forall n :: n in nodes ==> AVersionOfAKeyIsMet(b[i].servers[n].s.icache, b[i].servers[n].s.ccache, key, vc);
+    // assert forall s :: s in b[i].servers ==> AVersionOfAKeyIsMet(s.s.icache, s.s.ccache, key, vc);
+    assert |b[i].servers| == Nodes;
+    // assume |nodes| == Nodes;
+    assert forall j :: 0 <= j < |b[i].servers| ==> j in nodes;
+    assert forall j :: 0 <= j < |b[i].servers| ==> AVersionOfAKeyIsMet(b[i].servers[j].s.icache, b[i].servers[j].s.ccache, key, vc);
+}
 
-// this one can be proved, but the last requires is not passed at the end of lemma_PropagationAtTail
-// but this requires is ture, beacuse it can pass at the middle of lemma_PropagationAtTail
-lemma {:axiom} lemma_DepsIsMetForAllNodes(
-    b:Behavior<CMState>,
-    i:int,
-    nodes:seq<int>,
-    deps:Dependency
-)
-    requires i > 0 
-    requires IsValidBehaviorPrefix(b, i)
-    // requires forall j :: 0 <= j < i ==> CMNext(b[j], b[j+1])
-    requires |b[i].servers| == Nodes
-    requires forall j :: 0 <= j < Nodes ==> ServerValid(b[i].servers[j].s)
-    requires DependencyValid(deps)
-    requires |nodes| > 1
-    requires forall j :: 0 <= j < |nodes| ==> 0 <= nodes[j] < Nodes 
-    requires forall j :: 0 <= j < |nodes| ==> DepsIsMet(b[i].servers[nodes[j]].s.icache, b[i].servers[nodes[j]].s.ccache, deps)
-    // requires forall j :: 0 <= j < Nodes ==> j in nodes
-    ensures AllVersionsInDepsAreMetOnAllServers(b, i, deps)
-// {
-//     reveal_AllVersionsInDepsAreMetOnAllServers();
-//     reveal_DepsIsMet();
-//     assert forall n :: n in nodes ==> DepsIsMet(b[i].servers[n].s.icache, b[i].servers[n].s.ccache, deps);
-//     assert |b[i].servers| == Nodes;
-//     assert forall j :: 0 <= j < |b[i].servers| ==> j in nodes;
-//     assert forall j :: 0 <= j < |b[i].servers| ==> DepsIsMet(b[i].servers[j].s.icache, b[i].servers[j].s.ccache, deps);
-//     assert AllVersionsInDepsAreMetOnAllServers(b, i, deps);
-// }
+// // this one can be proved, but the last requires is not passed at the end of lemma_PropagationAtTail
+// // but this requires is ture, beacuse it can pass at the middle of lemma_PropagationAtTail
+// lemma {:axiom} lemma_DepsIsMetForAllNodes(
+//     b:Behavior<CMState>,
+//     i:int,
+//     nodes:seq<int>,
+//     deps:Dependency
+// )
+//     requires i > 0 
+//     requires IsValidBehaviorPrefix(b, i)
+//     // requires forall j :: 0 <= j < i ==> CMNext(b[j], b[j+1])
+//     requires |b[i].servers| == Nodes
+//     requires forall j :: 0 <= j < Nodes ==> ServerValid(b[i].servers[j].s)
+//     requires DependencyValid(deps)
+//     requires |nodes| > 1
+//     requires forall j :: 0 <= j < |nodes| ==> 0 <= nodes[j] < Nodes 
+//     requires forall j :: 0 <= j < |nodes| ==> DepsIsMet(b[i].servers[nodes[j]].s.icache, b[i].servers[nodes[j]].s.ccache, deps)
+//     // requires forall j :: 0 <= j < Nodes ==> j in nodes
+//     ensures AllVersionsInDepsAreMetOnAllServers(b, i, deps)
+// // {
+// //     reveal_AllVersionsInDepsAreMetOnAllServers();
+// //     reveal_DepsIsMet();
+// //     assert forall n :: n in nodes ==> DepsIsMet(b[i].servers[n].s.icache, b[i].servers[n].s.ccache, deps);
+// //     assert |b[i].servers| == Nodes;
+// //     assert forall j :: 0 <= j < |b[i].servers| ==> j in nodes;
+// //     assert forall j :: 0 <= j < |b[i].servers| ==> DepsIsMet(b[i].servers[j].s.icache, b[i].servers[j].s.ccache, deps);
+// //     assert AllVersionsInDepsAreMetOnAllServers(b, i, deps);
+// // }
 
 lemma lemma_AVersionOfAKeyIsMetForNodes(
     b:Behavior<CMState>,
@@ -321,16 +325,16 @@ lemma lemma_ServerNextSatisfyNodesAreNext(id:int, next:int)
 
 }
 
-lemma {:axiom} lemma_NodesFormACircle(start:int, end:int, nodes:seq<int>)
-    requires 0 <= start < Nodes
-    requires 0 <= end < Nodes
-    requires |nodes| > 1
-    requires nodes[0] == start
-    requires nodes[|nodes|-1] == end
-    requires forall j :: 0 <= j < |nodes| ==> 0 <= nodes[j] < Nodes
-    requires forall j :: 0 <= j < |nodes| - 1 ==> NodesAreNext(nodes[j], nodes[j+1])
-    requires NodesAreNext(end, start)
-    ensures forall j :: 0 <= j < Nodes ==> j in nodes
+// lemma {:axiom} lemma_NodesFormACircle(start:int, end:int, nodes:seq<int>)
+//     requires 0 <= start < Nodes
+//     requires 0 <= end < Nodes
+//     requires |nodes| > 1
+//     requires nodes[0] == start
+//     requires nodes[|nodes|-1] == end
+//     requires forall j :: 0 <= j < |nodes| ==> 0 <= nodes[j] < Nodes
+//     requires forall j :: 0 <= j < |nodes| - 1 ==> NodesAreNext(nodes[j], nodes[j+1])
+//     requires NodesAreNext(end, start)
+//     ensures forall j :: 0 <= j < Nodes ==> j in nodes
 
 
 function CalNode(start:int, n:int) : (res:int)
