DistributedSystems/VerifiedDS/src/Dafny/Distributed/Protocol/CausalMesh/proof/propagation_lemma3.dfy
@@ -1,0 +1,237 @@
+include "../distributed_system.dfy"
+// include "causalcut.dfy"
+include "packet_sending.dfy"
+include "properties.dfy"
+// include "propagation_lemma.dfy"
+include "propagation_lemma2.dfy"
+include "../../../Common/Collections/Seqs.s.dfy"
+
+module CausalMesh_Proof_PropagationLemma3_i {
+import opened CausalMesh_Cache_i
+import opened CausalMesh_Message_i
+import opened CausalMesh_Types_i
+import opened Environment_s
+import opened CausalMesh_DistributedSystem_i
+import opened CausalMesh_Properties_i
+import opened CausalMesh_Proof_Actions_i
+import opened Temporal__Temporal_s
+import opened CausalMesh_proof_Assumptions_i
+import opened CausalMesh_Proof_Constants_i
+// import opened CausalMesh_Proof_PropagationLemma_i
+import opened CausalMesh_Proof_PropagationLemma2_i
+import opened CausalMesh_Proof_PacketSending_i
+import opened CausalMesh_Proof_Properties_i
+// import opened CausalMesh_Proof_MessageReadReply_i
+import opened Collections__Seqs_s
+import opened Collections__Maps_i
+import opened Collections__Maps2_s
+
+lemma lemma_PropagationAtTail2(
+    b:Behavior<CMState>,
+    i:int,
+    idx:int,
+    p:Packet,
+    ios:seq<CMIo>
+)
+    requires 0 < i 
+    requires IsValidBehaviorPrefix(b, i)
+    // requires forall j :: 0 <= j < i ==> CMNext(b[j], b[j+1])
+    requires CMNext(b[i-1], b[i])
+    requires forall j :: 0 < j <= i ==> AllWriteDepsAreMet(b, j)
+    requires 0 <= idx < Nodes
+    requires |ios| > 0
+    requires ios[0].LIoOpReceive?
+    requires p.msg.Message_Propagation?
+    requires p in b[i-1].environment.sentPackets
+    requires p.dst == idx
+    requires idx == b[i-1].servers[idx].s.id
+    requires ios[0].r == p
+    requires PacketValid(p)
+    requires p.msg.start == b[i-1].servers[idx].s.next
+    requires p.msg.round == 2
+    requires ReceivePropagate(b[i-1].servers[idx].s, b[i].servers[idx].s, p, ExtractSentPacketsFromIos(ios))
+    ensures AllVersionsInDepsAreMetOnAllServers(b, i, p.msg.meta.deps)
+{
+    var p := ios[0].r;
+    var s := b[i-1].servers[idx].s;
+    var s' := b[i].servers[idx].s;
+
+    assert p.msg.start == s.next;
+
+    assert 0 <= i - 1;
+    assert IsValidBehaviorPrefix(b, i-1);
+    assert forall j :: 0 <= j < i-1 ==> CMNext(b[j], b[j+1]);
+    // assert CMNext(b[i-2], b[i-1]);
+    assert CMNext(b[i-1], b[i]);
+    // assert CMNextCommon(b[i-1], b[i]);
+    assert forall j :: 0 <= j < Nodes ==> ServerValid(b[i-1].servers[j].s);
+    assert p.msg.Message_Propagation?;
+    assert CMInit(b[0]);
+    assert |b[i-1].servers| == Nodes;
+    assert p in b[i-1].environment.sentPackets;
+    assert PacketValid(p);
+
+    assert p.dst == idx;
+    assert idx == s.id;
+
+    var nodes := lemma_Propagation2(b, i-1, p);
+    assert |nodes| > 1;
+    assert nodes[0] == p.msg.start;
+    assert nodes[|nodes|-2] == p.src;
+    assert nodes[|nodes|-1] == p.dst;
+    assert forall j :: 0 <= j < |nodes| ==> 0 <= nodes[j] < Nodes;
+    assert forall j :: 0 <= j < |nodes| - 1 ==> NodesAreNext(nodes[j], nodes[j+1]);
+    assert forall j :: 0 <= j < |nodes| - 1 ==> AVersionOfAKeyIsMet(b[i-1].servers[nodes[j]].s.icache, b[i-1].servers[nodes[j]].s.ccache, p.msg.key, p.msg.meta.vc);
+    assert forall j :: 0 <= j < |nodes| - 1 ==> DepsIsMet(b[i-1].servers[nodes[j]].s.icache, b[i-1].servers[nodes[j]].s.ccache, p.msg.meta.deps);
+
+    lemma_ServerNextSatisfyNodesAreNext(s.id, s.next);
+    assert NodesAreNext(s.id, p.msg.start);
+    assert p.dst == s.id;
+    lemma_NodesFormACircle(p.msg.start, p.dst, nodes);
+    // assert forall j :: 0 <= j < Nodes ==> j in nodes;
+    assert NodesAreComplete(nodes);
+
+    var new_deps := p.msg.meta.deps;
+    var (new_icache, new_ccache) := PullDeps2(s.icache, s.ccache, new_deps);
+    
+
+    var new_ccache' := InsertIntoCCache(new_ccache, p.msg.meta);
+    var new_icache' := AddMetaToICache(new_icache, p.msg.meta);
+    // reveal_DepsIsMet();
+    lemma_AddMetaToCacheImpliesMetaIsMetInNewCache(new_icache, new_ccache, p.msg.meta);
+    assert DepsIsMet(new_icache', new_ccache', p.msg.meta.deps);
+
+    assert VCHappendsBefore(p.msg.meta.vc, new_ccache'[p.msg.key].vc) || VCEq(p.msg.meta.vc, new_ccache'[p.msg.key].vc);
+    // reveal_DepsIsMet();
+    // lemma_DepsIsMet(b[i].servers[idx].s.icache, b[i].servers[idx].s.ccache, p.msg.meta.deps); // this could be proved, but may timeout
+    
+    lemma_AVersionOfAKeyIsMetIsTransitive(b, i, p.msg.key, p.msg.meta.vc, p.msg.meta.deps, nodes);
+    // assert forall j :: 0 <= j < |nodes| - 1 ==> AVersionOfAKeyIsMet(b[i].servers[nodes[j]].s.icache, b[i].servers[nodes[j]].s.ccache, p.msg.key, p.msg.meta.vc);
+    // assert forall j :: 0 <= j < |nodes| - 1 ==> DepsIsMet(b[i].servers[nodes[j]].s.icache, b[i].servers[nodes[j]].s.ccache, p.msg.meta.deps);
+    // assert forall j :: 0 <= j < |nodes| - 1 ==> AVersionOfAKeyIsMet(b[i].servers[nodes[j]].s.icache, b[i].servers[nodes[j]].s.ccache, p.msg.key, p.msg.meta.vc);
+    assert nodes[|nodes|-1] == idx;
+    
+    lemma_DepsIsMetForNodes(b, i, nodes, p.msg.meta.deps);
+
+    assert |b[i].servers| == Nodes;
+    assert forall j :: 0 <= j < Nodes ==> ServerValid(b[i].servers[j].s);
+    assert |nodes| > 1;
+    assert forall j :: 0 <= j < |nodes| ==> 0 <= nodes[j] < Nodes;
+    // lemma_Nodes(nodes);
+    // assert forall j :: 0 <= j < Nodes ==> j in nodes;
+    lemma_DepsIsMetForAllNodes(b, i, nodes, p.msg.meta.deps);
+    assert AllVersionsInDepsAreMetOnAllServers(b, i, p.msg.meta.deps);
+}
+
+predicate {:opaque} NodesAreComplete(
+    nodes:seq<int>
+)
+{
+    forall j :: 0 <= j < Nodes ==> j in nodes
+}
+
+lemma lemma_AddMetaToCacheImpliesMetaIsMetInNewCache(
+    icache:ICache,
+    ccache:CCache,
+    meta:Meta
+)
+    requires ICacheValid(icache)
+    requires CCacheValid(ccache)
+    requires MetaValid(meta)
+    requires forall k :: k in meta.deps ==> k in icache
+    requires forall k :: k in Keys_domain ==> k in icache && k in ccache
+    ensures var icache' := AddMetaToICache(icache, meta);
+            var ccache' := InsertIntoCCache(ccache, meta);
+            DepsIsMet(icache', ccache', meta.deps)
+{
+    reveal_DepsIsMet();
+    lemma_ReceiveAPropagationImpliesTheDepsAreAlreadyMet(icache, ccache, meta.deps);
+
+    var icache' := AddMetaToICache(icache, meta);
+    var ccache' := InsertIntoCCache(ccache, meta);
+    assert meta in icache'[meta.key];
+    assert VCHappendsBefore(meta.vc, ccache'[meta.key].vc) || VCEq(meta.vc, ccache'[meta.key].vc);
+    // assert forall k :: k in meta.deps ==> VCHappendsBefore(meta.deps[k], ccache'[k].vc) || VCEq(meta.deps[k], ccache'[k].vc);
+    assert DepsIsMet(icache', ccache', meta.deps);
+    // forall k | k in meta.deps 
+    // {
+    //     var vc := meta.deps[k];
+    //     var m := FoldMetaSet2(ccache'[k], icache'[k]);
+    //     assert VCEq(vc, m.vc) || VCHappendsBefore(vc, m.vc);
+    // }
+}
+
+
+lemma lemma_ServerNextSatisfyNodesAreNext(id:int, next:int)
+    requires 0 <= id < Nodes
+    requires next == Circle(id, Nodes)
+    ensures NodesAreNext(id, next)
+{
+
+}
+
+lemma {:axiom} lemma_NodesFormACircle(start:int, end:int, nodes:seq<int>)
+    requires 0 <= start < Nodes
+    requires 0 <= end < Nodes
+    requires |nodes| > 1
+    requires nodes[0] == start
+    requires nodes[|nodes|-1] == end
+    requires forall j :: 0 <= j < |nodes| ==> 0 <= nodes[j] < Nodes
+    requires forall j :: 0 <= j < |nodes| - 1 ==> NodesAreNext(nodes[j], nodes[j+1])
+    requires NodesAreNext(end, start)
+    // ensures forall j :: 0 <= j < Nodes ==> j in nodes
+    ensures NodesAreComplete(nodes)
+
+
+lemma lemma_DepsIsMetForNodes(
+    b:Behavior<CMState>,
+    i:int,
+    nodes:seq<int>,
+    deps:Dependency
+)
+    requires i > 0 
+    requires IsValidBehaviorPrefix(b, i)
+    requires |b[i].servers| == Nodes
+    requires forall j :: 0 <= j < Nodes ==> ServerValid(b[i].servers[j].s)
+    requires DependencyValid(deps)
+    requires |nodes| > 1
+    requires forall j :: 0 <= j < |nodes| ==> 0 <= nodes[j] < Nodes 
+    requires forall j :: 0 <= j < |nodes| - 1 ==> DepsIsMet(b[i].servers[nodes[j]].s.icache, b[i].servers[nodes[j]].s.ccache, deps)
+    requires DepsIsMet(b[i].servers[nodes[|nodes|-1]].s.icache, b[i].servers[nodes[|nodes|-1]].s.ccache, deps)
+    ensures forall j :: 0 <= j < |nodes| ==> DepsIsMet(b[i].servers[nodes[j]].s.icache, b[i].servers[nodes[j]].s.ccache, deps)
+{
+
+}
+
+// this one can be proved, but the last requires is not passed at the end of lemma_PropagationAtTail
+// but this requires is ture, beacuse it can pass at the middle of lemma_PropagationAtTail
+lemma lemma_DepsIsMetForAllNodes(
+    b:Behavior<CMState>,
+    i:int,
+    nodes:seq<int>,
+    deps:Dependency
+)
+    requires i > 0 
+    requires IsValidBehaviorPrefix(b, i)
+    // requires forall j :: 0 <= j < i ==> CMNext(b[j], b[j+1])
+    requires |b[i].servers| == Nodes
+    requires forall j :: 0 <= j < Nodes ==> ServerValid(b[i].servers[j].s)
+    requires DependencyValid(deps)
+    requires |nodes| > 1
+    requires forall j :: 0 <= j < |nodes| ==> 0 <= nodes[j] < Nodes 
+    requires forall j :: 0 <= j < |nodes| ==> DepsIsMet(b[i].servers[nodes[j]].s.icache, b[i].servers[nodes[j]].s.ccache, deps)
+    // requires forall j :: 0 <= j < Nodes ==> j in nodes
+    requires NodesAreComplete(nodes)
+    ensures AllVersionsInDepsAreMetOnAllServers(b, i, deps)
+{
+    reveal_AllVersionsInDepsAreMetOnAllServers();
+    reveal_DepsIsMet();
+    reveal_NodesAreComplete();
+    assert forall n :: n in nodes ==> DepsIsMet(b[i].servers[n].s.icache, b[i].servers[n].s.ccache, deps);
+    assert |b[i].servers| == Nodes;
+    assert forall j :: 0 <= j < |b[i].servers| ==> j in nodes;
+    assert forall j :: 0 <= j < |b[i].servers| ==> DepsIsMet(b[i].servers[j].s.icache, b[i].servers[j].s.ccache, deps);
+    assert AllVersionsInDepsAreMetOnAllServers(b, i, deps);
+}
+
+}
