DistributedSystems/VerifiedDS/src/Dafny/Distributed/Protocol/CausalMesh/proof/read_deps_is_met.dfy
@@ -22,6 +22,7 @@ import opened CausalMesh_Proof_Properties_i
 import opened CausalMesh_Proof_DepsAreMet_i
 import opened CausalMesh_Proof_ReadReplyIsMet_i
 import opened CausalMesh_Proof_ClientsAreMet_i
+import opened CausalMesh_Proof_AllwaysMet_i
 import opened Collections__Seqs_s
 import opened Collections__Maps_i
 import opened Collections__Maps2_s
