DistributedSystems/VerifiedDS/src/Dafny/Distributed/Protocol/CausalMesh/proof/read_reply_is_met.dfy
@@ -23,6 +23,7 @@ import opened CausalMesh_Proof_Properties_i
 import opened CausalMesh_Proof_DepsAreMet_i
 import opened CausalMesh_Proof_Monotonic_Read_i
 import opened CausalMesh_Proof_Environment_i
+import opened CausalMesh_Proof_AllwaysMet_i
 import opened Collections__Seqs_s
 import opened Collections__Maps_i
 import opened Collections__Maps2_s
@@ -281,9 +282,9 @@ lemma lemma_ServerReadReplyIsMetOnAllServers(
     requires ReceiveRead(b[i-1].servers[idx].s, b[i].servers[idx].s, p, sp)
     requires AllVersionsInCCacheAreMetOnAllServers(b, i-1, b[i-1].servers[idx].s.ccache)
     requires AllVersionsInDepsAreMetOnAllServers(b, i-1, p.msg.deps_read)
-    requires ServerNextDoesNotDecreaseVersions(b[i-1], b[i])
+    // requires ServerNextDoesNotDecreaseVersions(b[i-1], b[i])
     requires forall j :: 0 < j <= i ==> AllWriteDepsAreMet(b, j)
-
+    requires forall j :: 0 <= j < i ==> ServerNextDoesNotDecreaseVersions(b[j], b[j+1])
     ensures AllVersionsInCCacheAreMetOnAllServers(b, i, b[i].servers[idx].s.ccache)
     ensures AllVersionsInDepsAreMetOnAllServers(b, i, sp[0].msg.deps_rreply)
     ensures AVersionIsMetOnAllServers(b, i, sp[0].msg.key_rreply, sp[0].msg.vc_rreply)
@@ -371,101 +372,142 @@ lemma lemma_VersionMetIsTransitive(
 // }
 
 
-lemma {:axiom} lemma_AVersionIsMetWillAlwaysMet(
-    i1:ICache,
-    i2:ICache,
-    c1:CCache,
-    c2:CCache,
-    k:Key,
-    vc:VectorClock
-)
-    requires ICacheValid(i1)
-    requires ICacheValid(i2)
-    requires CCacheValid(c1)
-    requires CCacheValid(c2)
-    requires ICacheDoesNotDecrease(i1, i2)
-    requires CCacheDoesNotDecrease(c1, c2)
-    requires forall k :: k in Keys_domain ==> k in i1 && k in i2 && k in c1 && k in c2
-    requires k in Keys_domain
-    requires VectorClockValid(vc)
-    requires AVersionOfAKeyIsMet(i1, c1, k, vc)
-    ensures AVersionOfAKeyIsMet(i2, c2, k, vc)
+// lemma {:axiom} lemma_AVersionIsMetWillAlwaysMet(
+//     i1:ICache,
+//     i2:ICache,
+//     c1:CCache,
+//     c2:CCache,
+//     k:Key,
+//     vc:VectorClock
+// )
+//     requires ICacheValid(i1)
+//     requires ICacheValid(i2)
+//     requires CCacheValid(c1)
+//     requires CCacheValid(c2)
+//     requires ICacheDoesNotDecrease(i1, i2)
+//     requires CCacheDoesNotDecrease(c1, c2)
+//     requires forall k :: k in Keys_domain ==> k in i1 && k in i2 && k in c1 && k in c2
+//     requires k in Keys_domain
+//     requires VectorClockValid(vc)
+//     requires AVersionOfAKeyIsMet(i1, c1, k, vc)
+//     ensures AVersionOfAKeyIsMet(i2, c2, k, vc)
+// // {
+// //     var m1 := FoldMetaSet2(c1[k], i1[k]);
+// //     var m2 := FoldMetaSet2(c2[k], i2[k]);
+// //     assume VCEq(m1.vc, m2.vc) || VCHappendsBefore(m1.vc, m2.vc);
+// // }
+
+// lemma lemma_AVersionIsMetOnAllServersWillAlwaysMet(
+//     b:Behavior<CMState>,
+//     i:int,
+//     k:Key,
+//     vc:VectorClock
+// )
+//     requires 1 < i
+//     requires IsValidBehaviorPrefix(b, i)
+//     requires CMNext(b[i-1], b[i])
+//     requires CMNext(b[i-2], b[i-1])
+//     requires k in Keys_domain
+//     requires VectorClockValid(vc)
+//     requires AVersionIsMetOnAllServers(b, i-1, k, vc)
+//     requires ServerNextDoesNotDecreaseVersions(b[i-1], b[i])
+//     ensures AVersionIsMetOnAllServers(b, i, k, vc)
 // {
-//     var m1 := FoldMetaSet2(c1[k], i1[k]);
-//     var m2 := FoldMetaSet2(c2[k], i2[k]);
-//     assume VCEq(m1.vc, m2.vc) || VCHappendsBefore(m1.vc, m2.vc);
+//     assert forall j :: 0 <= j < |b[i-1].servers| ==> 
+//         CCacheDoesNotDecrease(b[i-1].servers[j].s.ccache, b[i].servers[j].s.ccache) 
+//         && ICacheDoesNotDecrease(b[i-1].servers[j].s.icache, b[i].servers[j].s.icache);
+    
+//     forall j | 0 <= j < |b[i].servers| 
+//         ensures AVersionOfAKeyIsMet(b[i].servers[j].s.icache, b[i].servers[j].s.ccache, k, vc)
+//     {
+//         assert AVersionOfAKeyIsMet(b[i-1].servers[j].s.icache, b[i-1].servers[j].s.ccache, k, vc);
+//         assert CCacheDoesNotDecrease(b[i-1].servers[j].s.ccache, b[i].servers[j].s.ccache);
+//         assert ICacheDoesNotDecrease(b[i-1].servers[j].s.icache, b[i].servers[j].s.icache);
+//         assert ServerValid(b[i-1].servers[j].s);
+//         assert ServerValid(b[i].servers[j].s);
+//         lemma_AVersionIsMetWillAlwaysMet(
+//             b[i-1].servers[j].s.icache,
+//             b[i].servers[j].s.icache,
+//             b[i-1].servers[j].s.ccache,
+//             b[i].servers[j].s.ccache,
+//             k,
+//             vc
+//         );
+//         assert AVersionOfAKeyIsMet(b[i].servers[j].s.icache, b[i].servers[j].s.ccache, k, vc);
+//     }
 // }
 
-lemma lemma_AVersionIsMetOnAllServersWillAlwaysMet(
-    b:Behavior<CMState>,
-    i:int,
-    k:Key,
-    vc:VectorClock
-)
-    requires 1 < i
-    requires IsValidBehaviorPrefix(b, i)
-    requires CMNext(b[i-1], b[i])
-    requires CMNext(b[i-2], b[i-1])
-    requires k in Keys_domain
-    requires VectorClockValid(vc)
-    requires AVersionIsMetOnAllServers(b, i-1, k, vc)
-    requires ServerNextDoesNotDecreaseVersions(b[i-1], b[i])
-    ensures AVersionIsMetOnAllServers(b, i, k, vc)
-{
-    assert forall j :: 0 <= j < |b[i-1].servers| ==> 
-        CCacheDoesNotDecrease(b[i-1].servers[j].s.ccache, b[i].servers[j].s.ccache) 
-        && ICacheDoesNotDecrease(b[i-1].servers[j].s.icache, b[i].servers[j].s.icache);
+// lemma lemma_AllVersionsInDepsAreMetOnAllServersWillAlwaysMet(
+//     b:Behavior<CMState>,
+//     i:int,
+//     deps:Dependency
+// )
+//     requires 1 < i
+//     requires IsValidBehaviorPrefix(b, i)
+//     requires CMNext(b[i-1], b[i])
+//     // requires CMNext(b[i-2], b[i-1])
+//     requires DependencyValid(deps)
+//     requires ServerNextDoesNotDecreaseVersions(b[i-1], b[i])
+//     requires AllVersionsInDepsAreMetOnAllServers(b, i-1, deps)
+//     ensures AllVersionsInDepsAreMetOnAllServers(b, i, deps)
+// {
+//     lemma_BehaviorValidImpliesOneStepValid(b, i-1);
+//     reveal_AllVersionsInDepsAreMetOnAllServers();
+//     assert forall j :: 0 <= j < |b[i-1].servers| ==> 
+//         CCacheDoesNotDecrease(b[i-1].servers[j].s.ccache, b[i].servers[j].s.ccache) 
+//         && ICacheDoesNotDecrease(b[i-1].servers[j].s.icache, b[i].servers[j].s.icache);
     
-    forall j | 0 <= j < |b[i].servers| 
-        ensures AVersionOfAKeyIsMet(b[i].servers[j].s.icache, b[i].servers[j].s.ccache, k, vc)
-    {
-        assert AVersionOfAKeyIsMet(b[i-1].servers[j].s.icache, b[i-1].servers[j].s.ccache, k, vc);
-        assert CCacheDoesNotDecrease(b[i-1].servers[j].s.ccache, b[i].servers[j].s.ccache);
-        assert ICacheDoesNotDecrease(b[i-1].servers[j].s.icache, b[i].servers[j].s.icache);
-        assert ServerValid(b[i-1].servers[j].s);
-        assert ServerValid(b[i].servers[j].s);
-        lemma_AVersionIsMetWillAlwaysMet(
-            b[i-1].servers[j].s.icache,
-            b[i].servers[j].s.icache,
-            b[i-1].servers[j].s.ccache,
-            b[i].servers[j].s.ccache,
-            k,
-            vc
-        );
-        assert AVersionOfAKeyIsMet(b[i].servers[j].s.icache, b[i].servers[j].s.ccache, k, vc);
-    }
-}
+//     forall k | k in deps 
+//         ensures AVersionIsMetOnAllServers(b, i, k, deps[k])
+//     {
+//         assert AVersionIsMetOnAllServers(b, i-1, k, deps[k]);
+//         lemma_AVersionIsMetOnAllServersWillAlwaysMet(b, i, k, deps[k]);
+//         assert AVersionIsMetOnAllServers(b, i, k, deps[k]);
+//     }
+// }
 
-lemma lemma_AllVersionsInDepsAreMetOnAllServersWillAlwaysMet(
-    b:Behavior<CMState>,
-    i:int,
-    deps:Dependency
-)
-    requires 1 < i
-    requires IsValidBehaviorPrefix(b, i)
-    requires CMNext(b[i-1], b[i])
-    // requires CMNext(b[i-2], b[i-1])
-    requires DependencyValid(deps)
-    requires ServerNextDoesNotDecreaseVersions(b[i-1], b[i])
-    requires AllVersionsInDepsAreMetOnAllServers(b, i-1, deps)
-    ensures AllVersionsInDepsAreMetOnAllServers(b, i, deps)
-{
-    lemma_BehaviorValidImpliesOneStepValid(b, i-1);
-    reveal_AllVersionsInDepsAreMetOnAllServers();
-    assert forall j :: 0 <= j < |b[i-1].servers| ==> 
-        CCacheDoesNotDecrease(b[i-1].servers[j].s.ccache, b[i].servers[j].s.ccache) 
-        && ICacheDoesNotDecrease(b[i-1].servers[j].s.icache, b[i].servers[j].s.icache);
+// // lemma {:axiom} lemma_AllDepsInICacheAreMetOnAllServersWillAlwaysMet(
+// //     b:Behavior<CMState>,
+// //     i:int,
+// //     idx:int
+// // )
+// //     requires 1 < i
+// //     requires IsValidBehaviorPrefix(b, i)
+// //     requires CMNext(b[i-1], b[i])
+// //     // requires CMNext(b[i-2], b[i-1])
+// //     requires 0 <= idx < Nodes
+// //     requires ServerNextDoesNotDecreaseVersions(b[i-1], b[i])
+// //     requires AllDepsInICacheAreMetOnAllServers(b, i-1, b[i].servers[idx].s.icache)
+// //     ensures AllDepsInICacheAreMetOnAllServers(b, i, b[i].servers[idx].s.icache)
+// // {
+// //     assert forall j :: 0 <= j < |b[i-1].servers| ==> 
+// //         CCacheDoesNotDecrease(b[i-1].servers[j].s.ccache, b[i].servers[j].s.ccache) 
+// //         && ICacheDoesNotDecrease(b[i-1].servers[j].s.icache, b[i].servers[j].s.icache);
     
-    forall k | k in deps 
-        ensures AVersionIsMetOnAllServers(b, i, k, deps[k])
-    {
-        assert AVersionIsMetOnAllServers(b, i-1, k, deps[k]);
-        lemma_AVersionIsMetOnAllServersWillAlwaysMet(b, i, k, deps[k]);
-        assert AVersionIsMetOnAllServers(b, i, k, deps[k]);
-    }
-}
+// //     var icache := b[i].servers[idx].s.icache;
+// //     assert ICacheValid(icache);
+// //     assert AllDepsInICacheAreMetOnAllServers(b, i-1, icache);
 
-// lemma {:axiom} lemma_AllDepsInICacheAreMetOnAllServersWillAlwaysMet(
+// //     forall k | k in icache
+// //     {
+// //         forall m:Meta | m in icache[k] 
+// //         {
+// //             forall kk | kk in m.deps 
+// //                 ensures AVersionIsMetOnAllServers(b, i, kk, m.deps[kk])
+// //             {
+// //                 assert AVersionIsMetOnAllServers(b, i-1, kk, m.deps[kk]);
+// //                 lemma_AVersionIsMetOnAllServersWillAlwaysMet(b, i, kk, m.deps[kk]);
+// //                 assert AVersionIsMetOnAllServers(b, i, kk, m.deps[kk]);
+// //             }
+// //         }
+// //     }
+
+// //     assert forall k :: k in icache ==>
+// //             forall m:Meta :: m in icache[k] ==> 
+// //                 forall kk :: kk in m.deps ==> AVersionIsMetOnAllServers(b, i, kk, m.deps[kk]);
+// // }
+
+// lemma lemma_AllVersionsInCCacheAreMetOnAllServersWillAlwaysMet(
 //     b:Behavior<CMState>,
 //     i:int,
 //     idx:int
@@ -476,69 +518,28 @@ lemma lemma_AllVersionsInDepsAreMetOnAllServersWillAlwaysMet(
 //     // requires CMNext(b[i-2], b[i-1])
 //     requires 0 <= idx < Nodes
 //     requires ServerNextDoesNotDecreaseVersions(b[i-1], b[i])
-//     requires AllDepsInICacheAreMetOnAllServers(b, i-1, b[i].servers[idx].s.icache)
-//     ensures AllDepsInICacheAreMetOnAllServers(b, i, b[i].servers[idx].s.icache)
+//     requires AllVersionsInCCacheAreMetOnAllServers(b, i-1, b[i].servers[idx].s.ccache)
+//     ensures AllVersionsInCCacheAreMetOnAllServers(b, i, b[i].servers[idx].s.ccache)
 // {
+//     assert i-1 > 0;
+//     assert IsValidBehaviorPrefix(b, i-1);
+//     lemma_BehaviorValidImpliesOneStepValid(b, i-1);
+//     reveal_AllVersionsInCCacheAreMetOnAllServers();
 //     assert forall j :: 0 <= j < |b[i-1].servers| ==> 
 //         CCacheDoesNotDecrease(b[i-1].servers[j].s.ccache, b[i].servers[j].s.ccache) 
 //         && ICacheDoesNotDecrease(b[i-1].servers[j].s.icache, b[i].servers[j].s.icache);
-    
-//     var icache := b[i].servers[idx].s.icache;
-//     assert ICacheValid(icache);
-//     assert AllDepsInICacheAreMetOnAllServers(b, i-1, icache);
 
-//     forall k | k in icache
+//     var ccache := b[i].servers[idx].s.ccache;
+
+//     forall k | k in ccache
+//         ensures AVersionIsMetOnAllServers(b, i, k, ccache[k].vc)
+//         ensures AllVersionsInDepsAreMetOnAllServers(b, i, ccache[k].deps)
 //     {
-//         forall m:Meta | m in icache[k] 
-//         {
-//             forall kk | kk in m.deps 
-//                 ensures AVersionIsMetOnAllServers(b, i, kk, m.deps[kk])
-//             {
-//                 assert AVersionIsMetOnAllServers(b, i-1, kk, m.deps[kk]);
-//                 lemma_AVersionIsMetOnAllServersWillAlwaysMet(b, i, kk, m.deps[kk]);
-//                 assert AVersionIsMetOnAllServers(b, i, kk, m.deps[kk]);
-//             }
-//         }
+//         assert AVersionIsMetOnAllServers(b, i-1, k, ccache[k].vc);
+//         lemma_AVersionIsMetOnAllServersWillAlwaysMet(b, i, k, ccache[k].vc);
+//         lemma_AllVersionsInDepsAreMetOnAllServersWillAlwaysMet(b, i, ccache[k].deps);
 //     }
-
-//     assert forall k :: k in icache ==>
-//             forall m:Meta :: m in icache[k] ==> 
-//                 forall kk :: kk in m.deps ==> AVersionIsMetOnAllServers(b, i, kk, m.deps[kk]);
 // }
-
-lemma lemma_AllVersionsInCCacheAreMetOnAllServersWillAlwaysMet(
-    b:Behavior<CMState>,
-    i:int,
-    idx:int
-)
-    requires 1 < i
-    requires IsValidBehaviorPrefix(b, i)
-    requires CMNext(b[i-1], b[i])
-    // requires CMNext(b[i-2], b[i-1])
-    requires 0 <= idx < Nodes
-    requires ServerNextDoesNotDecreaseVersions(b[i-1], b[i])
-    requires AllVersionsInCCacheAreMetOnAllServers(b, i-1, b[i].servers[idx].s.ccache)
-    ensures AllVersionsInCCacheAreMetOnAllServers(b, i, b[i].servers[idx].s.ccache)
-{
-    assert i-1 > 0;
-    assert IsValidBehaviorPrefix(b, i-1);
-    lemma_BehaviorValidImpliesOneStepValid(b, i-1);
-    reveal_AllVersionsInCCacheAreMetOnAllServers();
-    assert forall j :: 0 <= j < |b[i-1].servers| ==> 
-        CCacheDoesNotDecrease(b[i-1].servers[j].s.ccache, b[i].servers[j].s.ccache) 
-        && ICacheDoesNotDecrease(b[i-1].servers[j].s.icache, b[i].servers[j].s.icache);
-
-    var ccache := b[i].servers[idx].s.ccache;
-
-    forall k | k in ccache
-        ensures AVersionIsMetOnAllServers(b, i, k, ccache[k].vc)
-        ensures AllVersionsInDepsAreMetOnAllServers(b, i, ccache[k].deps)
-    {
-        assert AVersionIsMetOnAllServers(b, i-1, k, ccache[k].vc);
-        lemma_AVersionIsMetOnAllServersWillAlwaysMet(b, i, k, ccache[k].vc);
-        lemma_AllVersionsInDepsAreMetOnAllServersWillAlwaysMet(b, i, ccache[k].deps);
-    }
-}
 
 
 }
